Switch over to a more algebraic semantics

src/Spec/Proc.v
@@ -1,3 +1,5 @@
+Require Import Helpers.RelationAlgebra.
+
 Global Set Implicit Arguments.
 Global Generalizable Variables T R Op State.
 Global Set Printing Projections.
@@ -7,12 +9,13 @@ Inductive proc (Op: Type -> Type) (T : Type) : Type :=
 | Prim (op : Op T)
 | Ret (v : T)
 | Bind (T1 : Type) (p1 : proc Op T1) (p2 : T1 -> proc Op T).
+Arguments Prim {Op T}.
 Arguments Ret {Op T} v.
 
 (** Semantics: defined using big-step execution relations *)
 
-Definition OpSemantics Op State := forall T, Op T -> State -> T -> State -> Prop.
-Definition CrashSemantics State := State -> State -> Prop.
+Definition OpSemantics Op State := forall T, Op T -> relation State T.
+Definition CrashSemantics State := relation State unit.
 
 Record Dynamics Op State :=
   { step: OpSemantics Op State;
@@ -27,83 +30,33 @@ Section Dynamics.
 
   (** First, we define semantics of running programs with halting (without the
   effect of a crash or recovery) *)
-  Inductive Result State T :=
-  | Finished (v:T) (s:State)
-  | Crashed (s:State).
 
-  Arguments Crashed {State T}.
-  Arguments Prim {Op T}.
+  Fixpoint exec T (p: proc T) : relation State T :=
+    match p with
+    | Ret v => pure v
+    | Prim op => step op
+    | Bind p p' => and_then (exec p) (fun v => exec (p' v))
+    end.
 
-  Inductive exec : forall T, proc T -> State -> Result State T -> Prop :=
-  (* normal execution *)
-  | ExecRet : forall T (v:T) s,
-      exec (Ret v) s (Finished v s)
-  | ExecBindFinished : forall T T' (p: proc T) (p': T -> proc T')
-                         s v s' r,
-      exec p s (Finished v s') ->
-      exec (p' v) s' r ->
-      exec (Bind p p') s r
-  | ExecOp : forall T (op: Op T) s v s',
-      step op s v s' ->
-      exec (Prim op) s (Finished v s')
+  Fixpoint exec_crash T (p: proc T) : relation State unit :=
+    match p with
+    | Ret v => pure tt
+    | Prim op => rel_or (pure tt) (step op;; pure tt)
+    | Bind p p' => rel_or (pure tt)
+                         (rel_or (exec_crash p)
+                                 (and_then (exec p)
+                                           (fun v => exec_crash (p' v))))
+    end.
 
-  (* crashing (halting) execution *)
-  | ExecCrashBegin : forall T (p: proc T) s,
-      exec p s (Crashed s)
-  | ExecCrashEnd : forall T (p: proc T) s v s',
-      exec p s (Finished v s') ->
-      exec p s (Crashed s')
-  | ExecBindCrashed : forall T T' (p: proc T) (p': T -> proc T')
-                        s s',
-      exec p s (Crashed s') ->
-      exec (Bind p p') s (Crashed s')
-  .
+  Definition exec_recover R (rec: proc R) : relation State R :=
+    seq_star (crash_step;; exec_crash rec);;
+             (crash_step;; exec rec).
 
-
-  (* [exec_recover] models running recovery with crashes during recovery;
-      it's essentially
-    (crash_step; exec recovery -> crash)*;  // crashes during recovery
-    crash_step; exec recovery -> finished   // eventually recovery runs to completion
-   *)
-  Inductive exec_recover R (rec:proc R) (s:State) : R -> State -> Prop :=
-  | ExecRecoverExec : forall v s' s'',
-      crash_step s s' ->
-      exec rec s' (Finished v s'') ->
-      exec_recover rec s v s''
-  | ExecRecoverCrashDuringRecovery : forall s' v s'' s''',
-      crash_step s s' ->
-      exec rec s' (Crashed s'') ->
-      exec_recover rec s'' v s''' ->
-      exec_recover rec s v s'''
-  .
-
-  Inductive RResult T R :=
-  | RFinished (v:T) (s:State)
-  | Recovered (v:R) (s:State).
-
-  Arguments RFinished {T R} v s.
-  Arguments Recovered {T R} v s.
-
-  (* [rexec] combines the above. A program can execute in one of two ways:
-    - exec -> finish (producing RFinished)
-    - exec -> crash; exec_recover (producing Recovered)
-   *)
-  Inductive rexec T R : proc T -> proc R -> State -> RResult T R -> Prop :=
-  | RExec : forall (p:proc T) (rec:proc R) s v s',
-      exec p s (Finished v s') ->
-      rexec p rec s (RFinished v s')
-  | RExecCrash : forall (p:proc T) (rec:proc R) s s' rv s'',
-      exec p s (Crashed s') ->
-      exec_recover rec s' rv s'' ->
-      rexec p rec s (Recovered rv s'').
+  (* recovery execution *)
+  Definition rexec T R (p: proc T) (rec: proc R) : relation State R :=
+      exec_crash p;; exec_recover rec.
 
 End Dynamics.
 
 Notation "x <- p1 ; p2" := (Bind p1 (fun x => p2))
                             (at level 60, right associativity).
-
-Arguments exec {Op State} sem {T} p s r.
-Arguments Crashed {State T}.
-Arguments Prim {Op T}.
-Arguments RFinished {State T R} v s.
-Arguments Recovered {State T R} v s.
