src/Helpers/RelationAlgebra.v
@@ -1,0 +1,197 @@
+Require Import Helpers.Instances.
+Require Import Helpers.Helpers.
+Require Import Morphisms.
+
+Set Implicit Arguments.
+Generalizable All Variables.
+
+Section OutputRelations.
+
+  Context (A:Type).
+
+  (* an output relation: a homogenous relation over A that also emits some value
+  of type [T] *)
+  Definition relation T := A -> A -> T -> Prop.
+
+  Definition and_then {T1 T2} (r1: relation T1) (r2: T1 -> relation T2) :
+    relation T2 :=
+    fun x z o2 => exists o1 y, r1 x y o1 /\ (r2 o1) y z o2.
+
+  Definition seq {T1 T2} (r1: relation T1) (r2: relation T2)
+    : relation T2 :=
+    and_then r1 (fun _ => r2).
+
+  Definition fmap T1 T2 (f: T1 -> T2) (r:relation T1) : relation T2 :=
+    fun x y o => exists o0, r x y o0 /\ o = f o0.
+
+  Definition pure T (o0:T) : relation T :=
+    fun x y o => x = y /\ o = o0.
+
+  Definition map_out T1 T2 (f: T1 -> T2) : T1 -> relation T2 :=
+    fun v => fmap f (pure v).
+
+  Definition rel_or T (r1 r2: relation T) : relation T :=
+    fun x y o => r1 x y o \/ r2 x y o.
+
+  Inductive seq_star `(r: relation T) : relation T :=
+  | seq_star_refl : forall x o,
+      seq_star r x x o
+  | seq_star_one_more : forall x y z o1 o2,
+      r x y o1 ->
+      seq_star r y z o2 ->
+      seq_star r x z o2
+  .
+
+  Inductive bind_star `(r: T -> relation T) : T -> relation T :=
+  | bind_star_pure : forall (o:T) x y,
+      bind_star r o x y o
+  | bind_star_one_more : forall (o1:T) x y z o2 o3,
+      r o1 x y o2 ->
+      bind_star r o2 y z o3 ->
+      bind_star r o1 x z o3
+  .
+
+  Definition rimpl {T} (r1 r2: relation T) :=
+    forall x y o, r1 x y o -> r2 x y o.
+
+  Global Instance rimpl_preorder T : PreOrder (rimpl (T:=T)).
+  Proof.
+    unfold rimpl.
+    RelInstance_t; eauto.
+  Qed.
+
+  Definition requiv {T} (r1 r2: relation T) :=
+    forall x y o, r1 x y o <-> r2 x y o.
+
+  Infix "--->" := rimpl (at level 40, no associativity).
+  Infix "<--->" := requiv (at level 40, no associativity).
+
+  Global Instance rimpl_requiv_sub : subrelation (requiv (T:=T)) rimpl :=
+    ltac:(firstorder).
+
+  Global Instance requiv_equivalence : Equivalence (requiv (T:=T)) :=
+    RelInstance.
+
+  Hint Unfold Proper respectful pointwise_relation : t.
+  Hint Unfold seq and_then rel_or pure : t.
+
+  Ltac t :=
+    autounfold with t;
+    repeat match goal with
+           | |- _ <---> _ => split
+           | |- _ ---> _ => unfold "--->"
+           | [ H: ?r <---> _,
+                  H': ?r ?x ?y ?o |- _ ] =>
+             add_hypothesis (proj1 (H x y o) H')
+           | [ H: _ <---> ?r,
+                  H': ?r ?x ?y ?o |- _ ] =>
+             add_hypothesis (proj2 (H x y o) H')
+           | [ H: ?r ---> _,
+                  H': ?r ?x ?y ?o |- _ ] =>
+             add_hypothesis (H x y o H')
+           | _ => progress propositional
+           | _ => eauto 10
+        end.
+
+  Global Instance seq_respects_equiv :
+    Proper (requiv ==> requiv ==> requiv) (seq (T1:=T1) (T2:=T2)).
+  Proof.
+    t.
+  Qed.
+
+  Global Instance seq_respects_impl :
+    Proper (rimpl ==> rimpl ==> rimpl) (seq (T1:=T1) (T2:=T2)).
+  Proof.
+    t.
+  Qed.
+
+  Global Instance or_respects_equiv :
+    Proper (requiv ==> requiv ==> requiv) (rel_or (T:=T)).
+  Proof.
+    t.
+    (intuition idtac); t.
+    (intuition idtac); t.
+  Qed.
+
+  Global Instance or_respects_impl :
+    Proper (rimpl ==> rimpl ==> rimpl) (rel_or (T:=T)).
+  Proof.
+    t.
+    (intuition idtac); t.
+  Qed.
+
+  Theorem rel_or_introl T (r1 r2: relation T) :
+    r1 ---> rel_or r1 r2.
+  Proof.
+    t.
+  Qed.
+
+  Theorem rel_or_intror T (r1 r2: relation T) :
+    r2 ---> rel_or r1 r2.
+  Proof.
+    t.
+  Qed.
+
+  Theorem seq_assoc
+          `(r1: relation T1)
+          `(r2: relation T2)
+          `(r3: relation T3) :
+    seq (seq r1 r2) r3 <---> seq r1 (seq r2 r3).
+  Proof.
+    t.
+  Qed.
+
+  Theorem bind_left_id T1 T2 (v:T1) (r: T1 -> relation T2) :
+    and_then (pure v) r <---> r v.
+  Proof.
+    t.
+  Qed.
+
+  Theorem seq_left_id T1 T2 (v:T1) (r: relation T2) :
+    seq (pure v) r <---> r.
+  Proof.
+    unfold seq; apply bind_left_id.
+  Qed.
+
+  Theorem bind_assoc T1 T2 T3
+          (r1: relation T1)
+          (r2: T1 -> relation T2)
+          (r3: T2 -> relation T3) :
+    and_then (and_then r1 r2) r3 <--->
+             and_then r1 (fun v => and_then (r2 v) r3).
+  Proof.
+    t.
+  Qed.
+
+  Theorem bind_seq_assoc T1 T2 T3
+          (r1: relation T1)
+          (r2: T1 -> relation T2)
+          (r3: relation T3) :
+    seq (and_then r1 r2) r3 <--->
+             and_then r1 (fun v => seq (r2 v) r3).
+  Proof.
+    t.
+  Qed.
+
+  Theorem and_then_cong T1 T2 (r1 r1': relation T1) (r2 r2': T1 -> relation T2) :
+    r1 ---> r1' ->
+    (forall x, r2 x ---> r2' x) ->
+    and_then r1 r2 ---> and_then r1' r2'.
+  Proof.
+    t.
+    specialize (H0 o1); t.
+  Qed.
+
+  Global Instance and_then_respectful :
+    Proper (rimpl ==> pointwise_relation _ rimpl ==> rimpl) (and_then (T1:=T1) (T2:=T2)).
+  Proof.
+    unfold Proper, "==>"; intros.
+    apply and_then_cong; auto.
+  Qed.
+
+  Definition rimpl_refl T (r: relation T) : r ---> r := ltac:(reflexivity).
+  Definition requiv_refl T (r: relation T) : r <---> r := ltac:(reflexivity).
+
+End OutputRelations.
+
+Infix ";;" := seq (at level 21, left associativity).
