src/Spec/ProcTheorems.v
@@ -1,49 +1,47 @@
 Require Import Proc.
 Require Import Helpers.Instances.
+Require Import Helpers.RelationAlgebra.
 Require Import Helpers.Helpers.
-
-Local Notation "'exec_of!' p" := (exec _ p _ _) (at level 0, only parsing).
-Local Notation "'rexec_of!' p" := (rexec _ p _ _ _) (at level 0, only parsing).
-
-Ltac inv_exec :=
-  let t H := invertc H in
-  repeat match goal with
-         | [ H: exec_of! (Ret _) |- _ ] => t H
-         | [ H: exec_of! (Bind _ _) |- _ ] => t H
-         | [ H: exec_of! (Prim _) |- _ ] => t H
-         end.
-
-Ltac inv_rexec :=
-  match goal with
-  | [ H: rexec_of! _ |- _ ] => invert H
-  end.
 
 Section Dynamics.
   Context `(sem: Dynamics Op State).
   Notation proc := (proc Op).
   Notation step := sem.(step).
   Notation crash_step := sem.(crash_step).
+  Notation exec_crash := sem.(exec_crash).
   Notation exec := sem.(exec).
   Notation exec_recover := sem.(exec_recover).
   Notation rexec := sem.(rexec).
 
+  Hint Resolve rimpl_refl requiv_refl.
+
+  Theorem exec_to_crash T (p: proc T) :
+    rimpl (exec p;; pure tt) (exec_crash p).
+  Proof.
+    induction p; simpl in *.
+    - rewrite <- rel_or_intror.
+      reflexivity.
+    - rewrite seq_left_id.
+      reflexivity.
+    - rewrite <- rel_or_intror.
+      rewrite <- rel_or_intror.
+      rewrite bind_seq_assoc.
+      apply and_then_cong; auto.
+  Qed.
+
   Definition exec_equiv T (p p': proc T) :=
-    forall s r, exec p s r <-> exec p' s r.
+    requiv (exec p) (exec p').
 
   Global Instance exec_equiv_equiv T : Equivalence (exec_equiv (T:=T)) :=
     RelInstance.
 
   Infix "<==>" := exec_equiv (at level 99).
 
-  Hint Constructors Proc.exec.
-  Hint Constructors Proc.rexec.
-
   Theorem monad_left_id T T' (p: T' -> proc T) v :
       Bind (Ret v) p <==> p v.
   Proof.
-    split; intros.
-    - inv_exec; eauto.
-    - eauto.
+    unfold "<==>"; simpl.
+    rewrite bind_left_id; auto.
   Qed.
 
   Theorem monad_assoc
@@ -52,44 +50,8 @@ Section Dynamics.
           `(p3: T2 -> proc T3) :
     Bind (Bind p1 p2) p3 <==> Bind p1 (fun v => Bind (p2 v) p3).
   Proof.
-    split; intros.
-    - inv_exec; eauto.
-    - inv_exec; eauto.
-  Qed.
-
-  Definition rexec_equiv `(rec: proc R) T (p p': proc T) :=
-    forall s r,
-      rexec p rec s r <-> rexec p' rec s r.
-
-  Theorem exec_equiv_to_rexec `(rec: proc R) T (p p': proc T) :
-    exec_equiv p p' ->
-    rexec_equiv rec p p'.
-  Proof.
-    unfold rexec_equiv; split; intros.
-    - inv_rexec.
-      apply H in H1; eauto.
-      apply H in H1; eauto.
-    - inv_rexec.
-      apply H in H1; eauto.
-      apply H in H1; eauto.
-  Qed.
-
-  Instance exec_equiv_to_rexec_subr `(rec: proc R) :
-    subrelation (exec_equiv (T:=T)) (rexec_equiv rec (T:=T)).
-  Proof.
-    unfold subrelation; intros.
-    apply exec_equiv_to_rexec; auto.
-  Qed.
-
-  Theorem rexec_finish_any_rec
-          `(p: proc T)
-          `(rec: proc R) `(rec': proc R') :
-    forall s v s',
-      rexec p rec s (RFinished v s') ->
-      rexec p rec' s (RFinished v s').
-  Proof.
-    intros.
-    inv_rexec; eauto.
+    unfold "<==>"; simpl.
+    rewrite bind_assoc; auto.
   Qed.
 
   (* exec_recover (Bind p p') ==
@@ -100,19 +62,5 @@ Section Dynamics.
      (rexec (p' _) p -> recovered);
      exec (p' _) -> finish
 *)
-
-  Theorem exec_recover_bind_inv : forall `(p: proc R)
-                                    `(p': R -> proc R')
-                                    s rv' s'',
-      exec_recover (Bind p p') s rv' s'' ->
-      exists rv1 s1, exec_recover p s rv1 s1 /\
-                exists rv2 s2,
-                  kleene_star
-                    (fun '(rv, s) '(rv', s') =>
-                       rexec (p' rv) p s (Recovered rv' s'))
-                    (rv1, s1) (rv2, s2) /\
-                  exec (p' rv2) s2 (Finished rv' s'').
-  Proof.
-  Admitted.
 
 End Dynamics.
